temp saving

examples/count/verif.v
@@ -10,7 +10,7 @@ Require Import Poulet4.Semantics.
 Require Import Poulet4.SimplExpr.
 Require Import Poulet4.V1Model.
 Require Import ProD3.core.Hoare.
-Require Import ProD3.core.AssertionLang.
+(* Require Import ProD3.core.AssertionLang. *)
 
 Instance target : @Target Info (@Expression Info) := V1Model.
 
@@ -34,6 +34,39 @@ Definition init_es := Eval compute in snd instantiation.
 
 Notation ident := (P4String.t Info).
 Notation path := (list ident).
-
 Transparent IdentMap.empty IdentMap.set PathMap.empty PathMap.set.
+
+Module Experiment2.
+Definition this : path := [!"main"; !"ig"].
+Definition init_st : state := (PathMap.empty, init_es).
+
+(* 
+new_register *)
+
+Definition myFundef := Eval compute in
+  match PathMap.get [!"MyIngress"] ge with
+  | Some x => x
+  | None => dummy_fundef
+  end.
+
+Definition v1 : @ValueBase Info := ValBaseHeader [(!"firstBit", ValBaseBit 1%nat 0)] true.
+Definition v2 : @ValueBase Info := ValBaseStruct [(!"myHeader", v1)].
+Definition v3 : @ValueBase Info := ValBaseStruct [(!"counter", ValBaseBit 4%nat 0)].
+Definition v4 : @ValueBase Info := ValBaseStruct [(!"counter", ValBaseBit 4%nat 1)].
+Definition v5 : @ValueBase Info := ValBaseStruct [(!"egress_spec", ValBaseBit 9%nat 0)].
+Definition v6 : @ValueBase Info := ValBaseStruct [(!"egress_spec", ValBaseBit 9%nat 0)].
+
+Print init_es.
+
+
+(* {st' signal | exec_block [] inst_mem init_st myBlock st' signal }. *)
+Lemma eval_func: { st' & { signal | exec_func ge ge_typ ge_senum this inst_m init_st myFundef
+    [] [v2; v3; v5] st' [v2; v4; v6] signal} }.
+Proof.
+  repeat econstructor.
+  
+
+
+  solve [repeat econstructor].
+Defined.
 
